typeclass/typing/typeclass_tcexpScript.sml
@@ -8,26 +8,22 @@ open pure_cexpTheory;
 open typeclass_typesTheory typeclass_kindCheckTheory;
 val _ = new_theory "typeclass_tcexp";
 
+(* We associate a poly-type to variable.
+* This is needed for type elaboration.
+* It can be provided by the user as well. *)
+Type annot_cvname = ``:(cvname # (PredType_scheme option))``;
+
 Datatype:
   (* The first argument for each constructor is the type of the whole expression *)
-  tcexp = Var (PredType option) cvname                            (* variable                 *)
-          (* the first type is the type for the whole expression,
-          *  and the second type is the type for the operator *)
-        | Prim (PredType option) cop (tcexp list)                 (* primitive operations     *)
-        | App (PredType option) tcexp (tcexp list)                (* function application     *)
-          (* the types inside the list are the types assigned for
-          * the corresponding variables *)
-        | Lam (PredType option) ((PredType option # cvname) list)
-            tcexp                                                 (* lambda                   *)
-          (* the type scheme is the polymorphic type for
-          *  the binding expression. Used for inferencing *)
-        | Let (PredType option)
-             (PredType_scheme option) cvname tcexp tcexp          (* let                      *)
-        | Letrec (PredType option)
-            (((PredType_scheme option) # cvname # tcexp) list)
-            tcexp                                                 (* mutually recursive exps  *)
-        | NestedCase (PredType option) tcexp cvname cepat tcexp
-            ((cepat # tcexp) list)                                (* case of                  *)
+  (* So the user can do something like ``show ((read x)::Int)`` *)
+  tcexp = Var (type option) cvname                                   (* variable                 *)
+        | Prim (type option) cop (tcexp list)                        (* primitive operations     *)
+        | App (type option) tcexp (tcexp list)                       (* function application     *)
+        | Lam (type option) ((cvname # (type option)) list) tcexp    (* lambda                   *)
+        | Let (type option) annot_cvname tcexp tcexp                 (* let                      *)
+        | Letrec (type option) ((annot_cvname # tcexp) list) tcexp   (* mutually recursive exps  *)
+        | NestedCase (type option) tcexp cvname cepat tcexp
+            ((cepat # tcexp) list)                                   (* case of                  *)
 End
 
 (* top level declarations *)
@@ -53,6 +49,41 @@ Definition super_reachable_def:
       MEM dst c.super)
 End
 
+Theorem super_reachable_RULES:
+  (∀x y c. FLOOKUP cdb x = SOME c ∧ MEM y c.super ⇒
+    super_reachable cdb x y) ∧
+  (∀x y z. super_reachable cdb x y ∧ super_reachable cdb y z ⇒
+    super_reachable cdb x z)
+Proof
+  rw[super_reachable_def,relationTheory.TC_RULES] >>
+  metis_tac[cj 2 relationTheory.TC_RULES]
+QED
+
+Theorem super_reachable_SUBSET = cj 1 super_reachable_RULES;
+Theorem super_reachable_trans = cj 2 super_reachable_RULES;
+
+Theorem super_reachable_LEFT1_I:
+  ∀x y z c.
+    FLOOKUP cdb x = SOME c ∧ MEM y c.super ∧
+    super_reachable cdb y z ⇒
+    super_reachable cdb x z
+Proof
+  rw[] >> irule super_reachable_trans >>
+  first_x_assum $ irule_at Any >>
+  drule_all_then irule super_reachable_SUBSET
+QED
+
+Theorem super_reachable_RIGHT1_I:
+  ∀x y z c.
+    super_reachable cdb x y ∧
+    FLOOKUP cdb y = SOME c ∧ MEM z c.super ⇒
+    super_reachable cdb x z
+Proof
+  rw[] >> irule super_reachable_trans >>
+  first_x_assum $ irule_at Any >>
+  drule_all_then irule super_reachable_SUBSET
+QED
+
 Definition super_no_cycles_def:
   super_no_cycles cdb =
     ∀x. ¬(super_reachable cdb x x)
@@ -60,21 +91,14 @@ End
 
 Datatype:
   instinfo =
-    <| cstr : (mlstring # 'b) list (* class and type variable*)
-     (* ; class : mlstring *)
-     (* ; insttype : type *)
+    <| cstr : (mlstring # 'b) list (* class and type variable *)
+     ; nargs : num (* number of arguments to the type constructor *)
      ; impl : cvname |-> tcexp |> (* function name and its expression *)
 End
 
-Definition instinfo_constraint_ok_def:
-  instinfo_constraint_ok inst insttype =
-    !x. MEM x inst.cstr ==>
-      (* everything in the left must be in used in the right *)
-      SND x IN collect_type_vars insttype /\
-      (* everything in the left must be smaller than the type in the right *)
-      (* since we only allow a single type variable on the right now,
-      * so the following check should suffice *)
-      TypeVar (SND x) <> insttype
+Definition instinfo_well_scoped_def:
+  instinfo_well_scoped inf ⇔
+    (∀c v. MEM (c,v) inf.cstr ⇒ v < inf.nargs)
 End
 
 Definition instinfo_impl_ok:
@@ -82,8 +106,7 @@ Definition instinfo_impl_ok:
   ?c. FLOOKUP cdb class = SOME c /\
     (!meth ty. FLOOKUP c.methodsig meth = SOME ty ==>
       ?exp.
-       (FLOOKUP inst.impl meth = SOME exp
-       (* /\ TODO: check if the tcexp has the correct instantiated type *)) \/
+       FLOOKUP inst.impl meth = SOME exp \/
        FLOOKUP c.defaults meth = SOME exp) /\
     (?minimpl. !m.
       MEM minimpl c.minImp /\ MEM m minimpl ==>
@@ -91,15 +114,16 @@ Definition instinfo_impl_ok:
 End
 
 Definition freevars_tcexp_def[simp]:
-  freevars_tcexp (Var c v) = {v} /\
+  freevars_tcexp ((Var c v):tcexp) = {v} /\
   freevars_tcexp (Prim c op es) = BIGUNION (set (MAP (λa. freevars_tcexp a) es)) /\
   freevars_tcexp (App c e es) =
     freevars_tcexp e ∪ BIGUNION (set (MAP freevars_tcexp es)) ∧
-  freevars_tcexp (Lam c vs e) = freevars_tcexp e DIFF set (MAP SND vs) ∧
-  freevars_tcexp (Let c s v e1 e2) = freevars_tcexp e1 ∪ (freevars_tcexp e2 DELETE v) ∧
+  freevars_tcexp (Lam c vs e) = freevars_tcexp e DIFF set (MAP FST vs) ∧
+  freevars_tcexp (Let c v e1 e2) =
+    freevars_tcexp e1 ∪ (freevars_tcexp e2 DELETE (FST v)) ∧
   freevars_tcexp (Letrec c fns e) =
-    freevars_tcexp e ∪ BIGUNION (set (MAP (λ(s,fn,e). freevars_tcexp e) fns))
-      DIFF set (MAP (FST o SND) fns) ∧
+    freevars_tcexp e ∪ BIGUNION (set (MAP (λ(v,e). freevars_tcexp e) fns))
+      DIFF set (MAP (FST o FST) fns) ∧
   freevars_tcexp (NestedCase c g gv p e pes) =
     freevars_tcexp g ∪
     (((freevars_tcexp e DIFF cepat_vars p) ∪
@@ -117,8 +141,8 @@ Definition tcexp_wf_def[nocompute]:
     (∀m. op = AtomOp (Message m) ⇒ m ≠ "")) ∧
   tcexp_wf (App _ e es) = (tcexp_wf e ∧ EVERY tcexp_wf es ∧ es ≠ []) ∧
   tcexp_wf (Lam _ vs e) = (tcexp_wf e ∧ vs ≠ []) ∧
-  tcexp_wf (Let _ _ v e1 e2) = (tcexp_wf e1 ∧ tcexp_wf e2) ∧
-  tcexp_wf (Letrec _ fns e) = (EVERY tcexp_wf $ MAP (λx. SND (SND x)) fns ∧
+  tcexp_wf (Let _ v e1 e2) = (tcexp_wf e1 ∧ tcexp_wf e2) ∧
+  tcexp_wf (Letrec _ fns e) = (EVERY tcexp_wf $ MAP (λx. SND x) fns ∧
     tcexp_wf e ∧ fns ≠ []) ∧
   tcexp_wf (NestedCase _ g gv p e pes) = (
     tcexp_wf g ∧ tcexp_wf e ∧ EVERY tcexp_wf $ MAP SND pes ∧
@@ -133,9 +157,9 @@ End
 val tcexp_size_eq = fetch "-" "tcexp_size_eq";
 
 Theorem tcexp_size_lemma:
-  (∀xs s v e. MEM (s,v,e) xs ⇒ tcexp_size e < tcexp1_size xs) ∧
+  (∀xs v e. MEM (v,e) xs ⇒ tcexp_size e < tcexp1_size xs) ∧
   (∀xs p e. MEM (p,e) xs ⇒ tcexp_size e < tcexp3_size xs) ∧
-  (∀xs a. MEM a xs ⇒ tcexp_size a < tcexp6_size xs)
+  (∀xs a. MEM a xs ⇒ tcexp_size a < tcexp5_size xs)
 Proof
   rpt conj_tac
   \\ Induct \\ rw [] \\ fs [fetch "-" "tcexp_size_def"] \\ res_tac \\ fs []
@@ -144,11 +168,10 @@ QED
 Theorem better_tcexp_induction =
         TypeBase.induction_of “:tcexp”
           |> Q.SPECL [‘P’,
-                      ‘λxs. ∀s v e. MEM (s,v,e) xs ⇒ P e’,
-                      ‘λ(x,v,e). P e’,
+                      ‘λxs. ∀v e. MEM (v,e) xs ⇒ P e’,
+                      ‘λ(v,e). P e’,
                       ‘λlbs. ∀pat e. MEM (pat, e) lbs ⇒ P e’,
                       ‘λ(nm,e). P e’,
-                      ‘λ(p,e). P e’,
                       ‘λes. ∀e. MEM e es ⇒ P e’]
           |> CONV_RULE (LAND_CONV (SCONV [DISJ_IMP_THM, FORALL_AND_THM,
                                           pairTheory.FORALL_PROD,
@@ -165,11 +188,11 @@ Definition every_tcexp_def[simp]:
     (p (App a e es) ∧ every_tcexp p e ∧ EVERY (every_tcexp p) es) ∧
   every_tcexp p (Lam a vs e) =
     (p (Lam a vs e) ∧ every_tcexp p e) ∧
-  every_tcexp p (Let a s v e1 e2) =
-    (p (Let a s v e1 e2) ∧ every_tcexp p e1 ∧ every_tcexp p e2) ∧
+  every_tcexp p (Let a v e1 e2) =
+    (p (Let a v e1 e2) ∧ every_tcexp p e1 ∧ every_tcexp p e2) ∧
   every_tcexp p (Letrec a fns e) =
     (p (Letrec a fns e) ∧
-     every_tcexp p e ∧ EVERY (every_tcexp p) $ MAP (λx. SND (SND x)) fns) ∧
+     every_tcexp p e ∧ EVERY (every_tcexp p) $ MAP (λx. SND x) fns) ∧
   every_tcexp p (NestedCase a e1 v pat e2 rows) =
     (p (NestedCase a e1 v pat e2 rows) ∧
      every_tcexp p e1 ∧ every_tcexp p e2 ∧
