typeclass/typing/typeclass_unificationScript.sml
@@ -1136,20 +1136,6 @@ Proof
   qspecl_then  [`s`,`t1`,`t2`,`sx'`,`sx`] assume_tac pure_unify_mgu >> gvs[]
 QED
 
-(* How should I state it? *)
-Theorem pure_unify_preserve_kind:
-  kind_wf cdb vdb k t ∧ pure_wfs s ∧
-  pure_unify s (itype_of_scheme (ARB t) t) (itype_of t') = SOME s' ∧
-  ⇒ kind_wf cdb (ARB s' vdb) k t'
-Proof
-QED
-
-Theorem pure_apply_subst_preserve_kind:
-  kind_wf cdb vdb k t ∧ pure_wfs s ∧
-  ⇒
-  kind_wf cdb vdb k (pure_apply_subst s t)
-Proof
-QED
 (********************)
 
 val _ = export_theory();
